[sd] add Δsdt_m and update sd_example
Add 'per method' SDT context + relevant example from Nick

theories/sd_examples.v
@@ -12,22 +12,517 @@ From iris.algebra.lib Require Import gmap_view.
 
 From shack Require Import lang progdef subtype typing eval heap modality interp soundness.
 
-(* Will be updated soon with
-
-  <SDT where T = Dynamic>
-  class Box<T> {
-    private T $x;
-    <SDT when T <: dynamic >
-   public get(): T { return $this->x; }
-
-    <SDT when T:>dynamic>
-   public set(T $y): void { $this->x = $y; }
-   }
-
-<SDT when T<:dynamic>
-   class ROBox<+T> extends Box<T> {
-     <SDT>
-     public set(mixed $y): void { throw new Exception; }
-   }
-
+(*
+ * << SDT when T = Dynamic >>
+ * class Box<T> {
+ *   private T $x;
+ *
+ *   << SDT when T <: Dynamic >>
+ *   function get(): T { $ret = $this->x; return $ret; }
+ *
+ *   << SDT when T :> Dynamic >>
+ *   function set(T $y) : void { $this->x = $y; }
+ * }
  *)
+Definition Get := {|
+  methodname := "get";
+  methodargs := ∅;
+  methodrettype := GenT 0;
+  methodbody := GetC "$ret" ThisE "$x";
+  methodret := VarE "$ret";
+|}.
+
+Definition BoxSet := {|
+  methodname := "set";
+  methodargs := {["$y" := GenT 0 ]};
+  methodrettype := NullT;
+  methodbody := SetC ThisE "$x" (VarE "$y");
+  methodret := NullE;
+|}.
+
+Definition Box := {|
+  classname := "Box";
+  superclass := None;
+  generics := [Invariant];
+  constraints := [];
+  classfields := {["$x" := (Private, GenT 0)]};
+  classmethods := {["set" := BoxSet; "get" := Get]};
+|}.
+
+(*
+ * << SDT when T <: Dynamic >>
+ * class ROBox<+T> extends Box<T> {
+ *   << SDT when True >>
+ *   function set(mixed $y) : void { error }
+ * }
+ *)
+Definition ROBoxSet := {|
+  methodname := "set";
+  methodargs := {["$y" := MixedT ]};
+  methodrettype := NullT;
+  methodbody := ErrorC;
+  methodret := NullE;
+|}.
+
+Definition ROBox := {|
+  classname := "ROBox";
+  superclass := Some ("Box", [GenT 0]);
+  generics := [Covariant];
+  constraints := [];
+  classfields := ∅;
+  classmethods := {["set" := ROBoxSet ]};
+|}.
+
+Local Instance PDC : ProgDefContext := {
+  pdefs := {[ "ROBox" := ROBox; "Box" := Box ]};
+}.
+
+(* This is where we encode the <<SDT>> attribute *)
+Definition BoxSDT (σ: list lang_ty) :=
+  (subst_ty σ (GenT 0), DynamicT) :: (DynamicT, subst_ty σ (GenT 0)) :: [].
+
+Definition ROBoxSDT (σ: list lang_ty) :=
+  (subst_ty σ (GenT 0), DynamicT) :: [].
+
+Definition BoxGetSDT (σ: list lang_ty) :=
+  (subst_ty σ (GenT 0), DynamicT) :: [].
+
+Definition BoxSetSDT (σ: list lang_ty) :=
+  (DynamicT, subst_ty σ (GenT 0)) :: [].
+
+Definition ROBoxSetSDT (_: list lang_ty) : list constraint := [].
+
+Definition SDT (t: tag) (_ : list variance) (σ : list lang_ty) : list constraint :=
+  if String.eqb t "Box" then BoxSDT σ else
+  if String.eqb t "ROBox" then ROBoxSDT σ else
+  (IntT, BoolT) :: []
+.
+
+Definition SDT_M (t: tag) (m: string) (_ : list variance) (σ : list lang_ty) : list constraint :=
+  if String.eqb t "Box" && String.eqb m "get" then BoxGetSDT σ else
+  if String.eqb t "Box" && String.eqb m "set" then BoxSetSDT σ else
+  if String.eqb t "ROBox" && String.eqb m "set" then ROBoxSetSDT σ else
+  (IntT, BoolT) :: []
+.
+
+Local Instance SDTCC : SDTClassConstraints := {
+  Δsdt := SDT;
+  Δsdt_m := SDT_M;
+}.
+
+Local Instance SDTCP : SDTClassSpec.
+Proof.
+  split.
+  - move => A ? σ /Forall_lookup hwf.
+    apply Forall_lookup => k c.
+    rewrite /Δsdt /= /SDT.
+    destruct (A =? "Box")%string.
+    { rewrite /BoxSDT.
+      case : k => [ | [ | k]] /=.
+      - case => <-.
+        destruct (σ !! 0) as [ ty | ] eqn:h; last by split; constructor.
+        by apply hwf in h; split.
+      - case => <-.
+        destruct (σ !! 0) as [ ty | ] eqn:h; last by split; constructor.
+        by apply hwf in h; split.
+      - by rewrite lookup_nil.
+    }
+    destruct (A =? "ROBox")%string.
+    { rewrite /ROBoxSDT.
+      rewrite list_lookup_singleton.
+      case : k => [ | k] //=.
+      case => <-.
+      destruct (σ !! 0) as [ ty | ] eqn:h; last by split; constructor.
+      by apply hwf in h; split.
+    }
+    rewrite list_lookup_singleton.
+    case : k => [ | k] //=.
+    case => <-.
+    by split.
+  - admit.
+  - admit.
+  - admit.
+  - admit.
+  - admit.
+  - admit.
+  - admit.
+Admitted.
+
+Lemma has_fields_Box : has_fields "Box" {[ "$x" := (Private, GenT 0, "Box") ]}.
+Proof.
+  move => f vis fty orig; split => h.
+  - inv h.
+    + rewrite /pdefs /= lookup_insert_ne // lookup_insert in H.
+      simplify_eq.
+      rewrite /Box /= lookup_singleton_Some in H0.
+      by destruct H0 as [<- <-].
+    + by rewrite /pdefs /= lookup_insert_ne // lookup_insert in H; simplify_eq.
+  - rewrite lookup_singleton_Some in h.
+    destruct h as [<- [= <- <- <-]].
+    change Private with (Private, GenT 0).1.
+    by econstructor.
+Qed.
+
+Lemma has_fields_ROBox : has_fields "ROBox" {[ "$x" := (Private, GenT 0, "Box") ]}.
+Proof.
+  move => f vis fty orig; split => h.
+  - inv h.
+    + rewrite /pdefs /= lookup_insert in H.
+      by simplify_eq.
+    + rewrite /pdefs /= lookup_insert in H; simplify_eq.
+      rewrite /ROBox /= in H1.
+      case : H1 => ? <-.
+      subst.
+      move : has_fields_Box => hf.
+      apply hf in H2.
+      rewrite lookup_singleton_Some in H2.
+      case : H2 => <-.
+      by case => <- <- <-.
+  - rewrite lookup_singleton_Some in h.
+    destruct h as [<- [= <- <- <-]].
+    change (GenT 0) with (subst_ty [GenT 0] (GenT 0)).
+    eapply InheritsField => //.
+    change Private with (Private, GenT 0).1.
+    by econstructor.
+Qed.
+
+Lemma wf_extends_dyn : map_Forall wf_cdef_extends_dyn pdefs.
+Proof.
+  rewrite map_Forall_lookup => c0 d0.
+  rewrite lookup_insert_Some.
+  case => [[<- <-]|[?]].
+  { exists Box; split => //.
+    move => i c.
+    rewrite /Δsdt /= /SDT /ROBoxSDT /BoxSDT.
+    destruct ("ROBox" =? "Box")%string eqn:hfalse; first done.
+    destruct ("ROBox" =? "ROBox")%string eqn:hfalse_; last done.
+    rewrite /wf_cdef_extends_dyn_targs /=.
+    rewrite list_lookup_singleton_Some => [[? <-]] /=.
+    apply SubConstraint; by set_solver.
+  }
+  rewrite lookup_insert_Some.
+  case => [[? <-]|[?]] //.
+Qed.
+
+Lemma has_method_Box m o mdef:
+  has_method m "Box" o mdef →
+  (m = "get" ∧ o = "Box" ∧ mdef = Get) ∨
+  (m = "set" ∧ o = "Box" ∧ mdef = BoxSet).
+Proof.
+  move => h; inv h; last first.
+  { rewrite lookup_insert_ne // lookup_insert in H.
+    by simplify_eq.
+  }
+  rewrite lookup_insert_ne // lookup_insert in H.
+  simplify_eq.
+  rewrite lookup_insert_Some in H0.
+  case: H0 => [[? <-]|[?]].
+  - by firstorder.
+  - rewrite lookup_singleton_Some => h.
+    by firstorder.
+Qed.
+
+Lemma has_method_ROBox m o mdef:
+  has_method m "ROBox" o mdef →
+  (m = "get" ∧ o = "Box" ∧ mdef = subst_mdef [GenT 0] Get) ∨
+  (m = "set" ∧ o = "ROBox" ∧ mdef = ROBoxSet).
+Proof.
+  move => h; inv h.
+  - rewrite lookup_insert // in H.
+    simplify_eq.
+    rewrite lookup_singleton_Some in H0.
+    by firstorder.
+  - rewrite lookup_insert // in H.
+    simplify_eq.
+    rewrite /ROBox /= in H1, H0.
+    simplify_eq.
+    rewrite lookup_singleton_None in H0.
+    apply has_method_Box in H2.
+    case : H2 => [ [<- [<- <-]]| ].
+    { by left. }
+    by case => h; subst.
+Qed.
+
+Lemma wf_methods_dyn : map_Forall wf_cdef_methods_dyn_wf pdefs.
+Proof.
+  rewrite map_Forall_lookup => c0 d0.
+  rewrite lookup_insert_Some.
+  case => [[<- <-]|[?]].
+  { move => m o mdef hm.
+    apply has_method_ROBox in hm as [(-> & -> & ->) | (-> & -> & ->)].
+    - exists Box, [GenT 0]; split => //.
+      split; first by eauto.
+      move => i c /=.
+      rewrite list_lookup_singleton_Some.
+      case => ? <- /=.
+      constructor; by set_solver.
+    - exists ROBox, (gen_targs (length ROBox.(generics))); split => //.
+      split; first by constructor.
+      move => i c /=.
+      rewrite /SDT_M /ROBoxSetSDT /=.
+      by rewrite lookup_nil.
+  }
+  rewrite lookup_singleton_Some.
+  case => [<- <-].
+  move => m o mdef hm.
+  apply has_method_Box in hm as [(-> & -> & ->) | (-> & -> & ->)].
+  + exists Box, (gen_targs (length Box.(generics))); split => //.
+    split; first by constructor.
+    move => i c /=.
+    rewrite list_lookup_singleton_Some.
+    case => ? <-.
+    constructor; by set_solver.
+  + exists Box, (gen_targs (length Box.(generics))); split => //.
+    split; first by constructor.
+    move => i c /=.
+    rewrite list_lookup_singleton_Some.
+    case => ? <-.
+    constructor; by set_solver.
+Qed.
+
+Lemma wf_fields_dyn : map_Forall wf_cdef_fields_dyn_wf pdefs.
+Proof.
+  rewrite map_Forall_lookup => c0 d0.
+  rewrite lookup_insert_Some.
+  case => [[<- <-]|[?]].
+  { move => fields hf.
+    move : has_fields_ROBox => hf0.
+    rewrite (has_fields_fun _ _ _  hf hf0).
+    by apply map_Forall_singleton.
+  }
+  rewrite lookup_singleton_Some.
+  case => [<- <-].
+  move => fields hf.
+  move : has_fields_Box => hf0.
+  rewrite (has_fields_fun _ _ _  hf hf0).
+  by apply map_Forall_singleton.
+Qed.
+
+Lemma wf_mdefs_dyn : map_Forall cdef_wf_mdef_dyn_ty pdefs.
+Proof.
+  rewrite map_Forall_lookup => c0 d0.
+  rewrite lookup_insert_Some.
+  case => [[<- <-]|[?]].
+  { move => k m hm.
+    rewrite lookup_singleton_Some in hm.
+    case : hm => <- <-.
+    rewrite /ROBox /= /ROBoxSet /SDT_M /= /ROBoxSetSDT /wf_mdef_dyn_ty /=.
+    pose (Γ := {|
+        type_of_this := ("ROBox", gen_targs 1);
+        ctxt := to_dyn <$> {["$y" := MixedT]};
+      |}
+      ).
+    assert (wf_lty Γ).
+    { split => //.
+      - rewrite /this_type /=.
+        apply wf_ty_class with ROBox => //.
+        by apply gen_targs_wf_2.
+      - rewrite /Γ /=.
+        apply map_Forall_lookup => i ty.
+        rewrite lookup_fmap fmap_Some => [[ty0]].
+        rewrite lookup_singleton_Some.
+        by case => [[? <-]] ->.
+    }
+    exists Γ; split; first done.
+    split.
+    - constructor; first done.
+      constructor; first by repeat constructor.
+      apply map_Forall_lookup => i ty.
+      rewrite lookup_fmap fmap_Some => [[ty0]].
+      rewrite lookup_singleton_Some.
+      by case => [[? <-]] ->.
+    - apply ESubTy with NullT => //.
+      + by constructor.
+      + by constructor.
+      + apply SubTrans with SupportDynT; by eauto.
+  }
+  rewrite lookup_insert_Some.
+  case => [[<- <-]|[?]] //.
+  { move => k m hm.
+    rewrite lookup_insert_Some in hm.
+    case : hm => [[<- <-] | ].
+    - rewrite /wf_mdef_dyn_ty.
+      pose (Γ := {|
+        type_of_this := ("Box", gen_targs 1);
+        ctxt := to_dyn <$> {[ "$y" := GenT 0 ]};
+      |}
+      ).
+      assert (wf_lty Γ).
+      { split => //.
+        - rewrite /this_type /=.
+          apply wf_ty_class with Box => //.
+          by apply gen_targs_wf_2.
+        - rewrite /Γ /=.
+          apply map_Forall_lookup => i ty.
+          rewrite lookup_fmap fmap_Some => [[ty0]].
+          rewrite lookup_singleton_Some.
+          by case => [[? <-]] ->.
+      }
+      exists Γ; split; first done.
+      rewrite /BoxSet /= /SDT_M /= /BoxSetSDT /=.
+      split.
+      + eapply SetPrivTy => //.
+        * change Private with (Private, GenT 0).1.
+          by econstructor.
+        * apply ESubTy with DynamicT => //=.
+          { by constructor. }
+          { constructor. by lia. }
+          { by constructor. }
+          { apply SubConstraint.
+            by set_solver.
+          }
+      + apply ESubTy with NullT => //=.
+        * by constructor.
+        * by constructor.
+        * apply SubTrans with SupportDynT; by eauto.
+    - case => ?.
+      rewrite lookup_singleton_Some => [[<- <-]].
+      rewrite /wf_mdef_dyn_ty.
+      pose (Γ := {|
+        type_of_this := ("Box", gen_targs 1);
+        ctxt := {[ "$ret" := GenT 0 ]};
+      |}
+      ).
+      assert (wf_lty Γ).
+      { split => //.
+        - rewrite /this_type /=.
+          apply wf_ty_class with Box => //.
+          by apply gen_targs_wf_2.
+        - rewrite /Γ /=.
+          by apply map_Forall_singleton.
+      }
+      pose (Γ0 := {| type_of_this := ("Box", gen_targs 1); ctxt := to_dyn <$> ∅ |}).
+      exists Γ; split; first done.
+      rewrite /Get /= /SDT_M /= /BoxGetSDT /=.
+      split.
+      + replace Γ with (<[ "$ret" := subst_ty (gen_targs 1) (GenT 0)]> Γ0) ; last first.
+        { rewrite /Γ0 /Γ /= /local_tys_insert /=.
+          f_equal.
+          by rewrite fmap_empty insert_empty.
+        }
+        eapply GetPrivTy => //.
+        change Private with (Private, GenT 0).1.
+        by econstructor.
+      + apply ESubTy with (GenT 0) => //=.
+        * by constructor.
+        * by constructor.
+        * apply SubConstraint.
+          by set_solver.
+  }
+Qed.
+
+Lemma helper_ext: ∀ A B σ0, extends_using A B σ0 → A = "ROBox" ∧ B = "Box" ∧ σ0 = [GenT 0].
+Proof.
+  move => A B σ0 h; inv h.
+  rewrite /pdefs /= lookup_insert_Some in H.
+  destruct H as [[<- <-] | [? H]].
+  { split => //.
+    rewrite /ROBox /= in H0; by simplify_eq.
+  }
+  rewrite lookup_singleton_Some in H.
+  destruct H as [<- <-].
+  by rewrite /Box /= in H0.
+Qed.
+
+Lemma helper_in_Box : ∀ T σt, inherits_using "Box" T σt → T = "Box" ∧ σt = [GenT 0].
+Proof.
+  move => T σt h; inv h.
+  + rewrite /pdefs /=.
+    do 1 (rewrite lookup_insert_ne // in H).
+    rewrite lookup_insert in H.
+    by simplify_eq.
+  + apply helper_ext in H.
+    destruct H; discriminate.
+  + apply helper_ext in H.
+    destruct H; discriminate.
+Qed.
+
+Lemma helper_in: ∀ A B σ0, inherits_using A B σ0 →
+     (A = "Box" ∧ B = "Box" ∧ σ0 = [GenT 0]) ∨
+     (A = "ROBox" ∧ B = "Box" ∧ σ0 = [GenT 0]) ∨
+     (A = "ROBox" ∧ B = "ROBox" ∧ σ0 = [GenT 0]).
+Proof.
+  move => A B σ0 h.
+  inv h.
+  + rewrite /pdefs /=.
+    rewrite lookup_insert_Some in H.
+    destruct H as [[<- <-]|[? H]].
+    { by right; right. }
+    rewrite lookup_singleton_Some in H.
+    case : H => <- <-.
+    by left.
+  + apply helper_ext in H as [-> [-> ->]].
+    by right; left.
+  + apply helper_ext in H as [-> [-> ->]].
+    apply helper_in_Box in H0 as [-> ->].
+    by right; left.
+Qed.
+
+Lemma wf_override : wf_method_override pdefs.
+Proof.
+  move => A B adef bdef m σ0 mA mB hA hB hin hmA hmB.
+  apply helper_in in hin.
+  destruct hin as [[-> [-> ->]] | hin].
+  { rewrite /pdefs /= in hA, hB.
+    rewrite lookup_insert_ne // in hA.
+    rewrite lookup_insert_ne // in hB.
+    rewrite !lookup_insert in hA, hB.
+    simplify_eq.
+    change [GenT 0] with (gen_targs 1).
+    rewrite subst_mdef_gen_targs; first by apply mdef_incl_reflexive.
+    rewrite /Box /= in hmA.
+    rewrite lookup_insert_Some in hmA.
+    case: hmA => [[? <-] | ].
+    - rewrite /Box /BoxSet /=.
+      split => /=.
+      { apply map_Forall_singleton.
+        by repeat constructor.
+      }
+      split; first by constructor.
+      split; first by repeat constructor.
+      by repeat constructor.
+    - case => ?.
+      rewrite lookup_singleton_Some => [[? <-]].
+      split => /=; first by apply map_Forall_empty.
+      split; first by repeat constructor.
+      split; first by repeat constructor.
+      by repeat constructor.
+  }
+  destruct hin as [[-> [-> ->]] | hin].
+  { rewrite /pdefs /= in hA, hB.
+    rewrite lookup_insert in hA.
+    rewrite  lookup_insert_ne // lookup_insert in hB.
+    simplify_eq.
+    rewrite /ROBox /= lookup_singleton_Some in hmA.
+    destruct hmA as [<- <-].
+    rewrite /Box /= lookup_insert in hmB.
+    simplify_eq.
+    rewrite /ROBox /ROBoxSet /BoxSet /=.
+    split; last split => /=.
+    - by set_solver.
+    - move => k A B.
+      rewrite lookup_singleton_Some => [[<- <-]] /=.
+      rewrite lookup_fmap lookup_insert /= => [[<-]].
+      by eauto.
+    - by eauto.
+  }
+  destruct hin as [-> [-> ->]].
+  rewrite /pdefs /= in hA, hB.
+  rewrite !lookup_insert in hA, hB.
+  simplify_eq.
+  change [GenT 0] with (gen_targs 1).
+  rewrite subst_mdef_gen_targs; first by apply mdef_incl_reflexive.
+  rewrite /ROBox /= in hmA.
+  rewrite lookup_insert_Some in hmA.
+  case: hmA => [[? <-] | ].
+  - rewrite /ROBoxSet /=.
+    split => /=.
+    { apply map_Forall_singleton.
+      by repeat constructor.
+    }
+    split; first by constructor.
+    split; first by repeat constructor.
+    by repeat constructor.
+  - case => ?.
+    by rewrite lookup_empty.
+Qed.
